implicit type for rdf and triples, better consistency

src/Rdf.v
@@ -9,72 +9,70 @@ Section Rdf.
   Axiom todo_rdf: forall t, t.
 
   Record rdf_graph (I B L : Type):= mkRdfGraph {
-                                       graph : seq (triple I B L)
+                                       graph :> seq (triple I B L)
                                      }.
 
   Section PolyRdf.
     Variables I B L : Type.
+    Implicit Type g : rdf_graph I B L.
+    Implicit Type t : triple I B L.
+    Implicit Type ts : seq (triple I B L).
 
-    Definition empty_rdf_graph : rdf_graph I B L:= mkRdfGraph [::].
+    Definition empty_rdf_graph := mkRdfGraph [::] : rdf_graph I B L.
 
-    Definition is_ground(g : rdf_graph I B L) : bool :=
-      all (@is_ground_triple I B L) (graph g).
+    Definition is_ground g : bool :=
+      all (@is_ground_triple I B L) g.
 
     (* assumes shared identifier scope *)
-    Definition merge_rdf_graph (g h : rdf_graph I B L) : rdf_graph I B L :=
+    Definition merge_rdf_graph g1 g2 : rdf_graph I B L :=
       todo_rdf _.
 
     Definition merge_seq_rdf_graph (gs : seq (rdf_graph I B L)) : rdf_graph I B L :=
       foldr merge_rdf_graph empty_rdf_graph gs.
 
-    Definition add_triple (sg : option (rdf_graph I B L)) (t : (triple I B L)) : option (rdf_graph I B L).
-    Proof. destruct sg as [g |].
-           - destruct g as [g' sib ip ibl].
-             exact (Some {|
-                        graph := t :: g' ;
-                      |}).
+    Definition add_triple (og : option (rdf_graph I B L)) t : option (rdf_graph I B L).
+    Proof. destruct og as [[st] |].
+             exact (Some (mkRdfGraph (t :: st))).
            - exact None.
     Defined.
 
-    Definition relabeling_seq_triple (B' : Type) (μ : B -> B') (g : seq (triple I B L)) : seq (triple I B' L) :=
-      map (relabeling_triple μ) g.
+    Definition relabeling_seq_triple
+               (B' B'': Type) (μ : B' -> B'')
+               (ts : seq (triple I B' L)) : seq (triple _ B'' _) :=
+      map (relabeling_triple μ) ts.
 
     Section Relabeling_seq_triple.
       Variable B' : Type.
 
-      Lemma relabeling_seq_triple_comp_P (g1 g2 : seq (triple I B L)) (eqb : g1 = g2) (μ : B -> B') :
-        relabeling_seq_triple μ g1 = relabeling_seq_triple μ g2.
-      Proof. by rewrite eqb. Qed.
+      Lemma relabeling_seq_triple_ext (μ1 μ2 : B -> B') :
+        μ1 =1 μ2 -> forall ts, relabeling_seq_triple μ1 ts = relabeling_seq_triple μ2 ts.
+      Proof. move => μpqeq. elim=> [//|t ts' IHts] /=.
+             by rewrite IHts; f_equal; apply relabeling_triple_ext. Qed.
 
-      Lemma relabeling_seq_triple_comp (μ1 μ2 : B -> B) (g : seq (triple I B L)) : relabeling_seq_triple μ1 (relabeling_seq_triple μ2 g) = (relabeling_seq_triple μ1 \o (relabeling_seq_triple μ2)) g.
-      Proof. by []. Qed.
+      Lemma relabeling_seq_triple_comp (B'' : Type) (μ2 : B -> B') (μ1 : B' -> B'') ts :
+        relabeling_seq_triple μ1 (relabeling_seq_triple μ2 ts) = relabeling_seq_triple (μ1 \o μ2) ts.
+      Proof. by elim ts => [//| t ts' ihts] /=; rewrite relabeling_triple_comp ihts. Qed.
 
-      Lemma relabeling_seq_triple_ext (μ1 μ2 : B -> B') : μ1 =1 μ2 -> forall g : seq (triple I B L), relabeling_seq_triple μ1 g = relabeling_seq_triple μ2 g.
-      Proof. move => μpqeq. elim=> [//|h t IHt] /=. rewrite IHt. f_equal. by apply relabeling_triple_ext . Qed.
     End Relabeling_seq_triple.
 
-    Lemma relabeling_seq_triple_id (g : seq (triple I B L)) : relabeling_seq_triple id g = g.
-    Proof. elim g => [//| a l ihl] /=. by rewrite relabeling_triple_id ihl.
+    Lemma relabeling_seq_triple_id ts : relabeling_seq_triple id ts = ts.
+    Proof. by elim ts => [//| t ts' ihts] /= ; rewrite relabeling_triple_id ihts.
     Qed.
 
-    Lemma relabeling_seq_triple_comp_simpl (g : seq (triple _ _ _)) (μ12 μ23 : B -> B) :
-      relabeling_seq_triple (μ23 \o μ12) g = relabeling_seq_triple μ23 (relabeling_seq_triple μ12 g).
-    Proof. elim g => [//|h t iht] /=. by rewrite relabeling_triple_comp; f_equal; apply iht.
-    Qed.
-
-    Definition relabeling (B' : Type) (μ : B -> B') (g : rdf_graph I B L): rdf_graph I B' L:=
+    Definition relabeling
+               (B' B'' : Type) (μ : B' -> B'')
+               (g : rdf_graph I B' L) : rdf_graph I B'' L:=
       mkRdfGraph (relabeling_seq_triple μ (graph g)).
 
-    Lemma relabeling_comp (g : rdf_graph I B L) (μ12 μ23: B -> B) :
-      (relabeling μ23 \o (relabeling μ12)) g = relabeling (μ23 \o μ12) g.
-    Proof. by case g => g'; rewrite /relabeling relabeling_seq_triple_comp_simpl //=.
+    Lemma relabeling_comp (B' B'': Type) g (μ1 : B -> B') (μ2: B' -> B'') :
+      relabeling μ2 (relabeling μ1 g) = relabeling (μ2 \o μ1) g.
+    Proof. by case g => g'; rewrite /= /relabeling relabeling_seq_triple_comp.
     Qed.
-
 
     Section Relabeling_graph.
       Variable B' : Type.
 
-      Lemma relabeling_id (g : rdf_graph I B L) : relabeling id g = g.
+      Lemma relabeling_id g : relabeling id g = g.
       Proof. case g => g' /=. by rewrite /relabeling relabeling_seq_triple_id.
       Qed.
 
@@ -82,21 +80,19 @@ Section Rdf.
       Proof. move=> μpweq g. by case g=> g'; rewrite /relabeling (relabeling_seq_triple_ext μpweq). Qed.
 
     End Relabeling_graph.
-
-    Lemma relabeling_comp_simpl (μ1 μ2 : B -> B) (g : rdf_graph I B L) : relabeling μ1 (relabeling μ2 g) = relabeling (μ1 \o μ2) g.
-    Proof. by rewrite -relabeling_comp. Qed.
-
   End PolyRdf.
+
   Section EqRdf.
     Variables I B L : eqType.
+    Implicit Type g : rdf_graph I B L.
 
-    Definition eqb_rdf (g1 g2 : rdf_graph I B L) : bool :=
+    Definition eqb_rdf g1 g2 : bool :=
       (graph g1) == (graph g2).
 
-    Lemma eqb_rdf_refl (g : rdf_graph I B L) : eqb_rdf g g.
+    Lemma eqb_rdf_refl g : eqb_rdf g g.
     Proof. by rewrite /eqb_rdf. Qed.
 
-    Lemma eqb_rdf_symm (g1 g2 : rdf_graph I B L) : eqb_rdf g1 g2 = eqb_rdf g2 g1.
+    Lemma eqb_rdf_symm g1 g2 : eqb_rdf g1 g2 = eqb_rdf g2 g1.
     Proof. by rewrite /eqb_rdf. Qed.
 
     Definition rdf_eqP : Equality.axiom eqb_rdf.
@@ -108,68 +104,68 @@ Section Rdf.
 
     Canonical rdf_eqType := EqType (rdf_graph I B L) (EqMixin rdf_eqP).
 
-    Definition terms (g : rdf_graph I B L) : seq (term _ _ _) :=
+    Definition terms g : seq (term _ _ _) :=
       flatten (map (fun t => terms_triple t) (graph g)).
 
-    Definition bnodes (g : rdf_graph I B L) : seq (term _ _ _) :=
-      filter (fun t => is_bnode t) (terms g).
+    Definition bnodes g : seq (term _ _ _) :=
+      filter (@is_bnode I B L) (terms g).
 
-    Lemma bijective_eqb_rdf mu nu g1 g2 : cancel mu nu -> eqb_rdf g1 (relabeling mu g2) ->  eqb_rdf g2 (relabeling nu g1).
+    Lemma bijective_eqb_rdf mu nu g1 g2 :
+      cancel mu nu -> eqb_rdf g1 (relabeling mu g2) ->  eqb_rdf g2 (relabeling nu g1).
     Proof.
       move=> cancel_mu_nu. rewrite /eqb_rdf => /eqP /= ->.
-      rewrite -relabeling_seq_triple_comp_simpl. 
+      rewrite relabeling_seq_triple_comp.
       have /relabeling_seq_triple_ext-> : nu \o mu =1 id by [].
       rewrite relabeling_seq_triple_id; exact: eqb_rdf_refl.
     Qed.
 
-    Definition is_iso (g1 g2 : rdf_graph I B L) (μ : B -> B) :=
+    Definition is_iso g1 g2 (μ : B -> B) :=
       (bijective μ) /\ eqb_rdf g1 (relabeling μ g2).
 
-    Definition iso (g1 g2 : rdf_graph I B L) := exists (μ : B -> B),
+    Definition iso g1 g2 := exists (μ : B -> B),
         is_iso g1 g2 μ.
 
-    Lemma iso_refl (g : rdf_graph I B L) : iso g g.
+    Lemma iso_refl g : iso g g.
     Proof. rewrite /iso /is_iso; exists id; split.
            exists id => //.
            by rewrite relabeling_id eqb_rdf_refl.
     Qed.
 
-    Lemma iso_symm (g1 g2 : rdf_graph I B L) :
-      iso g1 g2 <-> iso g2 g1.
+    Lemma iso_symm g1 g2 : iso g1 g2 <-> iso g2 g1.
     Proof.
       rewrite /iso /is_iso.
       split; case=> mu [mu_bij heqb_rdf]; case: (mu_bij)=> [nu h1 h2];
                                                          (exists nu; split; [exact: bij_can_bij h1 | exact: bijective_eqb_rdf heqb_rdf]).
     Qed.
 
-    Lemma iso_trans (g1 g2 g3: rdf_graph I B L) : iso g1 g2 -> iso g2 g3 -> iso g1 g3.
+    Lemma iso_trans g1 g2 g3 : iso g1 g2 -> iso g2 g3 -> iso g1 g3.
     Proof. rewrite /iso/is_iso/eqb_rdf/relabeling => [[μ1 [bij1/eqP eqb1]] [μ2 [bij2/eqP eqb2]]].
            exists (μ1 \o μ2). split.
            by apply bij_comp.
-           by rewrite eqb1 eqb2 relabeling_seq_triple_comp_simpl. 
+           by rewrite eqb1 eqb2 relabeling_seq_triple_comp.
     Qed.
 
     Definition isocanonical_mapping (M : rdf_graph I B L -> rdf_graph I B L) :=
-      forall (g : rdf_graph I B L),
-        iso (M g) g /\ forall (h : rdf_graph I B L), iso (M g) (M h) <-> iso g h.
+      forall g1, iso (M g1) g1 /\
+              forall g2, iso (M g1) (M g2) <-> iso g1 g2.
 
   End EqRdf.
 
   Section CountRdf.
     Variables I B L : countType.
+    Implicit Type g : rdf_graph I B L.
 
-    Definition code_rdf (g : rdf_graph I B L) :=
-      let (g') := g in
-      GenTree.Node 0 (map (@code_triple I B L) g').
+    Definition code_rdf g :=
+      GenTree.Node 0 (map (@code_triple I B L) g).
 
     Definition decode_rdf (x : GenTree.tree nat) : option (rdf_graph I B L).
     Proof. destruct x.
            - exact None.
            - destruct n as [| n'].
-             + induction l as [| t ts IHts].
+             + induction l as [| gen gens IHgens].
                * exact (Some (mkRdfGraph [::])).
-               * destruct (@decode_triple I B L t) as [t'|].
-                 -- apply (@add_triple I B L IHts t').
+               * destruct (@decode_triple I B L gen) as [t'|].
+                 -- apply (@add_triple I B L IHgens t').
                  -- exact None.
              + exact None.
     Defined.
@@ -178,7 +174,7 @@ Section Rdf.
     Proof. case => g. rewrite /code_rdf /decode_rdf.
            induction g as [| t ts IHts].
            - by [].
-           - by rewrite /= cancel_triple_encode IHts. 
+           - by rewrite /= cancel_triple_encode IHts.
     Qed.
 
     Definition rdf_canChoiceMixin := PcanChoiceMixin cancel_rdf_encode.
